Use Fig. \ref{fig:tri_baudh} for all problems in this section.
\renewcommand{\theequation}{\theenumi}
\begin{enumerate}[label=\arabic*.,ref=\thesubsection.\theenumi]
\numberwithin{equation}{enumi}



\item  Show that
	\begin{equation}
	\cos \theta = \sin \brak{90\degree - \theta}
	\label{eq:tri_baudh_comp}	
	\end{equation}


\begin{figure}[!ht]
	\begin{center}
		\resizebox{\columnwidth}{!}{\input{./figs/triangle/tri_baudh.tex}}
	\end{center}
	\caption{Baudhayana Theorem}
	\label{fig:tri_baudh}	
\end{figure}


\solution From Problem \ref{prob:tri_compl_angle} and  \eqref{eq:tri_trig_defs}
%
\begin{multline}
\label{eq:tri_90-ang}
\cos \angle BAC = \cos \alpha =	\cos \brak{90\degree-\theta} = \frac{c}{b} 
\\
= \sin \angle ABC = \sin \theta
\end{multline}
%
\item
Show that 
%
\begin{equation}
\label{ch1_budh_basic}
b = a \cos \theta + c \sin \theta
\end{equation}
%
\solution We observe that
%
\begin{align}
BD &= a \cos \theta \\
AD &= c \cos\alpha = c \sin \theta \quad \brak{\text{From} \quad \eqref{eq:tri_90-ang}
}
\end{align}
%
Thus,
\begin{equation}
BD + AD = b = a \cos \theta + c \sin \theta
\end{equation}
\item
From \eqref{ch1_budh_basic}, show that
%
\begin{equation}
%
\label{eq:tri_sin_cos_id}
\sin ^2 \theta + \cos ^2 \theta = 1
\end{equation}


%
\solution Dividing both sides of \eqref{ch1_budh_basic} by $b$, 
\begin{align}
1 &= \frac{a}{b}\cos\theta + \frac{c}{b}\sin\theta\\
\Rightarrow &\sin ^2 \theta + \cos ^2 \theta = 1 \quad \brak{\text{from} \quad \eqref{eq:tri_trig_defs}}
\end{align}

\item
	Using \eqref{ch1_budh_basic}, show that
	\begin{equation}
	\label{eq:tri_baudh}
	c^2 = a^2 + b^2
	\end{equation}
	\eqref{eq:tri_baudh} is known as the Baudhayana theorem.  It is also known as the Pythagoras theorem.

\solution From \eqref{ch1_budh_basic},
\begin{align}
c &= a\frac{a}{c} + b \frac{b}{c} \quad \brak{\text{from} \quad \eqref{eq:tri_trig_defs}}\\
\Rightarrow c^2 &= a^2 + b^2
\end{align}
%
\item Show that $c > a, c > b$
%
\solution From 	\eqref{eq:tri_baudh},
	\begin{align}
	c^2 - a^2 &= b^2
\\
\implies c-a &= \frac{b^2}{c+a} > 0 
\\
\implies c &> a
	\end{align}
%
Similarly, it can be shown that $c > b$.
\item In a right angled triangle, the hypotenuse is the longest side.
\label{them:hyp_largest}
\item Draw Fig. \ref{fig:tri_baudh} for $a = 4, c =3$.
\label{const:tri_baudh}
%
\\
\solution Problem \ref{const:tri_right_angle} is used to draw $\triangle ABC$.
%
Using Problem \ref{prob:tri_polar},
\begin{align}
\vec{D} &= BD\myvec{\cos \alpha\\  \sin \alpha} 
&= a \sin \theta \myvec{ \sin \theta \\ \cos \theta } 
\label{eq:tri_baudh_foot}
\end{align}
%
Using \eqref{eq:tri_baudh_foot}, the python code for  Fig. \ref{fig:tri_baudh} is
\begin{lstlisting}
codes/triangle/tri_baudh.py
\end{lstlisting}
%
and the equivalent latex-tikz code is
%
\begin{lstlisting}
figs/triangle/tri_baudh.tex
\end{lstlisting}
%
\item Using 	\eqref{eq:tri_baudh}, for $a = 4, c = 3$,
%
\begin{align}
b = \sqrt{a^2+c^2} = \sqrt{4^2+3^2} = 5
\end{align}
%
\item For  point $\vec{D} = \myvec{d_1\\d_2}$, its {\em norm} is defined as
%
\begin{align}
OD = d_1^2+d_2^2 = \norm{\vec{D}} \define \sqrt{\vec{D}^T\vec{D}}, 
\label{eq:tri_norm_def}
\end{align}
%
where 
%
\begin{align}
\label{eq:tri_transpose_def}
 \vec{D}^T  \define \myvec{d_1 & d_2},
\\
\vec{D}^T\vec{D} \define \myvec{d_1 & d_2} \myvec{d_1 \\ d_2} = d_1^2+d_2^2
\end{align}
%
\eqref{eq:tri_transpose_def} is the definition of {\em transpose}. $\vec{D}$ is defined to be a {\em column vector} and $\vec{D}^T$  is the corresponding {\em row vector} representing the same point.

\item Also, it is easy to verify that
%
\begin{align}
\label{eq:tri_norm_dist}
AC \define  \norm{\vec{A}-\vec{C}} =  \norm{\myvec{4\\-3}} = \sqrt{3^2+4^2} = 5
\end{align}
%
This is known as the {\em distance formula}.
%
\item Prove the distance formula in \eqref{eq:tri_norm_dist} using Baudhayana theorem.
%
\item Show that 
\label{them:tri_baudh_orth}
\begin{align}
\label{eq:tri_baudh_orth}
\brak{\vec{A}-\vec{B}}^T\brak{\vec{B}-\vec{C}} = 0
\end{align}
\\
\solution From the Baudhayana theorem,
\begin{align}
a^2+c^2 &= b^2
\\
\implies \norm{\vec{B}-\vec{A}}^2+\norm{\vec{C}-\vec{A}}^2&=\norm{\vec{B}-\vec{C}}^2
\label{eq:tri_baudh_orth_norm}
\end{align}
which, from \eqref{eq:tri_transpose_def}
 can be expressed as
\begin{multline}
\brak{\vec{B}-\vec{A}}^T\brak{\vec{B}-\vec{A}}
+
\brak{\vec{C}-\vec{B}}^T\brak{\vec{C}-\vec{B}}
\\
=
\brak{\vec{A}-\vec{C}}^T\brak{\vec{A}-\vec{C}}
\end{multline}
%
Expanding
\begin{multline}
\brak{\vec{B}-\vec{A}}^T\brak{\vec{B}-\vec{A}} 
\\
= \vec{B}^T\vec{B} - \vec{B}^T\vec{A} - \vec{A}^T\vec{B}+\vec{A}^T\vec{A}
\end{multline}
$\because \vec{A}^T\vec{B} = \vec{B}^T\vec{A}$, the above equation can be expressed as
\begin{align}
\norm{\vec{B}-\vec{A}}^2 = 
\norm{\vec{A}}^2 + \norm{\vec{B}}^2 - 2\vec{A}^T\vec{B}
\end{align}
%
Thus, \eqref{eq:tri_baudh_orth_norm} can be expressed using the above equation as
\begin{multline}
\norm{\vec{A}}^2 + \norm{\vec{B}}^2 - 2\vec{A}^T\vec{B}
\\
+
\norm{\vec{B}}^2 + \norm{\vec{C}}^2 - 2\vec{B}^T\vec{C}
\\
=
\norm{\vec{A}}^2 + \norm{\vec{C}}^2 - 2\vec{A}^T\vec{C}
\end{multline}
%
which can be simplified to obtain
%
\begin{multline}
2\norm{\vec{B}}^2 - 2\vec{B}^T\vec{C}
\\
- 2\vec{A}^T\vec{B}+ 2\vec{A}^T\vec{C}
=0
\\
\text{or, } \vec{B}^T\brak{\vec{B}-\vec{C}}
-\vec{A}^T\brak{\vec{B}-\vec{C}} = 0
\\
\implies \brak{\vec{B}^T-\vec{A}^T}\brak{\vec{B}-\vec{C}} = 0
\end{multline}
yielding \eqref{eq:tri_baudh_orth}.

\end{enumerate}
